# Exercises: generating functions (1)

Find explicit formulas for the following sequences:
1. $a_{n+1} = 3a_n+2$ for $n\ge 0$, $a_0=0$

    <details>
    <summary>solution</summary>

    * $2x/(1-x)(1-3x)$
    * $3^n-1$
    </details>

2. $a_{n+1} = \alpha a_n + \beta$ for $n\ge 0$, $a_0=0$

    <details>
    <summary>solution</summary>

    * $\beta x/(1-x)(1-\alpha x)$
    * ${\alpha^n-1\over \alpha-1}\beta$
    </details>

3. $a_{n+1} = a_n/3 + 1$ for $n\ge 0$, $a_0=1$

    <details>
    <summary>solution</summary>

    * ${3/2\over 1-x}-{1/2\over 1-x/3}$
    * ${3^{n+1}-1\over 2\cdot 3^n}$
    </details>

4. $a_{n+2} = 2a_{n+1}-a_n$ for $n\ge 0$, $a_0=0$, $a_1=1$

    <details>
    <summary>solution</summary>

    * $x/(1-x)^2$;
    * $n$
    </details>

5. $a_{n+2} = 3a_{n+1}-2a_n+3$ for $n\ge 0$, $a_0=1$, $a_1=2$

    <details>
    <summary>solution</summary>

    * ${4\over 1-2x}-{3\over (1-x)^2}$
    * $2^{n+2}-3n-3$    </details>

6. $a_n = 2a_{n-1}-a_{n-2}+(-1)^n$ for $n>1$, $a_0=a_1=1$

    <details>
    <summary>solution</summary>

    * ${1/2\over (1-x)^2}+{1/4\over 1-x}+{1/4\over 1+x}$
    * ${2n+3+(-1)^n\over 4}$
    </details>

7. $a_n = 2a_{n-1}-n\cdot(-1)^n$ for $n\ge 1$, $a_0=0$

    <details>
    <summary>solution</summary>

    * ${x/9-2/9\over (1+x)^2}+{2/9\over 1-2x}$
    * ${2^{n+1}-(3n+2)(-1)^n\over 9}$
    </details>

8. $a_n = 3a_{n-1} + {n\choose 2}$ for $n\ge 1$, $a_0=2$

    <details>
    <summary>solution</summary>

    * $A(x) = \frac{-2x^3 + 7x^2 - 6x + 2}{(1-3x)(1-x)^3}$
    * ${1\over 8}(19\cdot 3^n-2n(n+2)-3)$
    </details>

9. $a_n = 2a_{n-1}-a_{n-2}-2$ for $n > 1$, $a_0=a_{10}=0$

    <details>
    <summary>solution</summary>

    * $A(x) = \frac{9x - 11 x^2}{(1-x)^3} = \frac{-11}{1-x} + \frac{13}{(1-x)^2} - \frac{2}{(1-x)^3}$
    * $n(a_1+1-n)$, so with $a_{10}$, $a_n=n(10-n)$
    </details>

10. $a_n = 4(a_{n-1}-a_{n-2})+(-1)^n$ for $n \ge 2$, $a_0=1$, $a_1=4$

    <details>
    <summary>solution</summary>

    * ${1+x+x^2\over (1+x)(1-2x)^2} = {1\over 9}{1\over 1+x} +\left({-5\over 18}\right) {1\over 1-2x} + \left({7\over 6}\right){1\over (1-2x)^2}$
    * ${1\over 9}(-1)^n-{5\over 18}\cdot 2^n+{7\over 6}(n+1)\cdot 2^n$
    </details>

11. $a_n = -3a_{n-1}+a_{n-2}+3a_{n-3}$ for $n\ge 3$, $a_0=20$, $a_1=-36$, $a_2=60$

    <details>
    <summary>solution</summary>

    * $A(x) = \frac{20 + 24x - 68x^2}{(1+3x)(1-x^2)}$
    * $5\cdot(-3)^n+18\cdot(-1)^n-3$
    </details>

12. $a_n = -3a_{n-1}+a_{n-2}+3a_{n-3}+128n$ for $n\ge 3$, $a_0=0$, $a_1=0$, $a_2=0$

    <details>
    <summary>solution</summary>

    * $A(x) = \frac{128 x^3 (3-2x)}{(1+3x)(1-x)^3(1+x)}$
    * $8n^2+28n-29-11(-3)^n+40(-1)^n$
    </details>

